\begin{definition}[Beta Function]
    \[
    B(\alpha, \beta) = \int^10 x^{\alpha - 1}(1 - x)^{\beta - 1} dx = \frac{\Gamma(\alpha)\Gamma(\beta)}{\Gamma(\alpha + \beta)}    
    \]
\end{definition}

\begin{definition}
    A random variable $X$ has a \emph{beta distribution with parameters} 
    $\alpha > 0$ and $\beta > 0$ iff. the density function of $X$ is
    \[
        f(x) =
        \begin{cases}
        \frac{x^{\alpha - 1}(1 - x)^{\beta - 1}}{B(\alpha, \beta)} &, 0 \leq x < 1,\\
        0&, \text{elsewhere}
        \end{cases} 
    \]
    where
    \[
        B(\alpha, \beta) = \int^1_0 x^{\alpha - 1}(1 - x)^{\beta - 1} dx
        = \frac{\Gamma(\alpha)\Gamma(\beta)}{\Gamma(\alpha + \beta)}
    \]
\end{definition}

\begin{theorem}[mean and variance of beta distribution]
    If a random variable $X$ has a gamma distribution with parameters $\alpha > 0$  and $\beta > 0$, then
    \[
    E(X) = \frac{\alpha}{\alpha + \beta} \text{ and } 
    V(X) = \frac{\alpha\beta}{(\alpha + \beta)^2(\alpha + \beta + 1)}
    \]
\end{theorem}
\begin{theorem}
    By definition \nameref{def:exp_val_cont},
    \begin{align*}
        E(X) &= \int_{-\infty}^{\infty} xf(x) dx \\
        &= \int^{1}_{0} x \cdot \frac{x^{\alpha - 1}(1 - x)^{\beta - 1}}{B(\alpha, \beta)} dx \\
        &= \frac{1}{B(\alpha, \beta)} \int^{1}_{0} x^\alpha(1 - x)^{\beta - 1} dx \\
        &= \frac{B(\alpha + 1, \beta)}{B(\alpha, \beta)} \\
        &= \frac{\Gamma(\alpha + 1)\Gamma(\beta)}{\Gamma(\alpha + \beta + 1)}   \times \frac{\Gamma(\alpha)\Gamma(\beta)}{\Gamma(\alpha + \beta)} \\
        &= \frac{\alpha \Gamma(\alpha)\Gamma(\beta)}{(\alpha + \beta)\Gamma(\alpha + \beta )}   \times \frac{\Gamma(\alpha)\Gamma(\beta)}{\Gamma(\alpha + \beta)} \\
        E(X) &= \frac{\alpha}{\alpha + \beta}
    \end{align*}
    Since variance $V(X) = E(X^2) - [E(X)]^2$,

    \begin{align*}
        E(X^2) &= \int^{1}_{0} x^2 \cdot \frac{x^{\alpha - 1}(1 - x)^{\beta - 1}}{B(\alpha, \beta)} dx \\
        &= \frac{1}{B(\alpha, \beta)} \int^{1}_{0} x^{\alpha + 1}(1 - x)^{\beta - 1} dx \\ 
        &= \frac{B(\alpha + 2, \beta)}{B(\alpha, \beta)} \\
        &= \frac{\Gamma(\alpha + 2)\Gamma(\beta)}{\Gamma(\alpha + \beta + 2)}   \times \frac{\Gamma(\alpha)\Gamma(\beta)}{\Gamma(\alpha + \beta)} \\
        &= \frac{\alpha(\alpha + 1)\Gamma(\alpha)\Gamma(\beta)}{(\alpha + \beta + 1)(\alpha + \beta)\Gamma(\alpha + \beta)}   \times \frac{\Gamma(\alpha)\Gamma(\beta)}{\Gamma(\alpha + \beta)} \\
        E(X^2) &= \frac{\alpha(\alpha + 1)}{(\alpha + \beta + 1)(\alpha + \beta)}
    \end{align*}

    Therefore,

    \begin{align*}
        V(X) &= E(X^2) - [E(X)]^2 \\
        &= \frac{\alpha(\alpha + 1)}{(\alpha + \beta + 1)(\alpha + \beta)} - {\left(\frac{\alpha}{\alpha + \beta}\right)}^2 \\
        &= \frac{\alpha(\alpha + 1)}{(\alpha + \beta + 1)(\alpha + \beta)} - \frac{\alpha^2}{(\alpha + \beta)^2}\\
        &= \frac{ (\alpha^2 + \alpha)(\alpha + \beta) - \alpha^2(\alpha + \beta + 1)}{(\alpha + \beta + 1)(\alpha + \beta)^2} \\
        &=  \frac{\alpha^2(\alpha + \beta) + \alpha(\alpha + \beta) - \alpha^2(\alpha + \beta) - \alpha^2}{(\alpha + \beta + 1)(\alpha + \beta)^2} \\
        &= \frac{\alpha^2 + \alpha\beta - \alpha^2}{(\alpha + \beta + 1)(\alpha + \beta)^2} \\
        &= \frac{\alpha\beta}{(\alpha + \beta + 1)(\alpha + \beta)^2}
    \end{align*}

\end{theorem}