\section{Poisson Distribution}
\begin{theorem}
    From calculus,
    \[
    e^x = 1 + \frac{x}{1!}  + \frac{x^2}{2!} + \frac{x^3}{3!} + \ldots = \sum^\infty_{n=0} \frac{x^n}{n!}
    \]
\end{theorem}
\begin{definition}
    A random variable $X$ has a \emph{Poisson probability distribution} iff.
    
    \[
    P(X=x) = \frac{\lambda^x}{x!}e^{-\lambda}, x = 0, 1, \ldots, \lambda > 0    
    \]
\end{definition}

\begin{corollary}\label{thm:poi_sum_to_one}
    For poisson random variable $X$, the following is true
    \[
    \sum_{\text{all } x} P(X = x) = \sum^\infty_{x = 0} \frac{\lambda^x}{x!}e^{-\lambda}   = 1
    \]
\end{corollary}
\begin{proof}
    \begin{align*}
    \sum^\infty_{x = 0} \frac{\lambda^x}{x!}e^{-\lambda} &= e^{-\lambda}\sum^\infty_{x = 0} \frac{\lambda^x}{x!} \\
    &= e^{-\lambda} \cdot e^{\lambda} \\
    &= 1
    \end{align*} 
\end{proof}

\begin{theorem}[mean and variance of poisson distribution]
    If $X$ is a random poisson distribution with parameter $\lambda$, then
    \[
        E(X) = \lambda \text{ and } V(X) = \lambda
    \]
\end{theorem}

\begin{proof}
    Note that the first term of the summands is 0,
    \begin{align*}
        E(X) &= \sum^\infty_{x = 0} x\frac{\lambda^x e^{-\lambda}}{x!}
        = \sum^\infty_{x = 1} x\frac{\lambda^x e^{-\lambda}}{x!} \\
        &= \sum^\infty_{x = 1} x\frac{\lambda \lambda^{x-1} e^{-\lambda}}{x(x-1)!} \\
        &= \lambda \sum^\infty_{x = 1} \frac{\lambda^{x-1} e^{-\lambda}}{(x-1)!}
    \end{align*}
    Let $z = x - 1$, then
    \[
        E(X) =\lambda \sum^\infty_{z = 0} \frac{\lambda^z e^{-\lambda}}{z!} = \lambda
    \]
    The latter summation is geometric distribution sum as in \nameref{thm:poi_sum_to_one}, then it is $1$.
    
    Note that the first 2 terms of the summands are 0,
    \begin{align*}
        E[X(X-1)] 
            &= \sum^\infty_{x = 0} x(x-1)\frac{\lambda^x e^{-\lambda}}{x!} \\
        E(X^2 - X)
            &= \sum^\infty_{x = 2} \frac{\lambda^x e^{-\lambda}}{(x-2)!} \\
        E(X^2) - E(X)   
            &= \lambda^2 \sum^\infty_{x = 2} \frac{\lambda^{x-2} e^{-\lambda}}{(x-2)!} \\
        \text{Let z = x - 2} \\
        E(X^2) - \lambda
            &= \lambda^2 \sum^\infty_{z = 0} \frac{\lambda^z e^{-\lambda}}{z!}
            = \lambda^2 (1) \\
        E(X^2) &= \lambda^2 + \lambda \\
        \therefore 
            V(X) &= E(X^2) - [E(X)^2] \\
                &= \lambda^2 + \lambda - (\lambda)^2 \\
            V(X)   &= \lambda
    \end{align*}
\end{proof}


